Fixed soundness proof of clstep

examples/litmus/theory/bir_promisingExecScript.sml
@@ -124,16 +124,15 @@ End
  * DESCRIPTION:
  *   Implements an executable version of the core-local read rule.
  *)
-Definition eval_clstep_read_def:
-  eval_clstep_read s M var a_e xcl acq rel =
+Definition eval_clstep_load_def:
+  eval_clstep_load s M var a_e xcl acq rel =
   case bir_eval_exp_view a_e s.bst_environ s.bst_viewenv of
   | (SOME l, v_addr) =>
       let
         (* Pre-view of the memory *)
-        v_pre = MAXL [ v_addr; s.bst_v_rNew;
-                       ifView (acq /\ rel) s.bst_v_Rel;
-                       ifView (acq /\ rel) (MAX s.bst_v_rOld s.bst_v_wOld)
-                     ];
+        v_pre = MAXL [v_addr; s.bst_v_rNew;
+                      ifView (acq /\ rel) s.bst_v_Rel;
+                      ifView (acq /\ rel) (MAX s.bst_v_rOld s.bst_v_wOld)];
         (* Get the readable writes/messages with timestamp *)
         msgs_ts  = mem_readable M l (MAX v_pre (s.bst_coh l)) 
       in
@@ -170,8 +169,8 @@ End
  * DESCRIPTION:
  *   Implements an executable version of the core-local fulfil rule.
  *)
-Definition eval_clstep_fulfil_def:
-  eval_clstep_fulfil p cid s M a_e v_e xcl acq rel =
+Definition eval_clstep_store_fulfil_def:
+  eval_clstep_store_fulfil p cid s M a_e v_e xcl acq rel =
   let
     (l_opt, v_addr) = bir_eval_exp_view a_e s.bst_environ s.bst_viewenv;
     (v_opt, v_data) = bir_eval_exp_view v_e s.bst_environ s.bst_viewenv
@@ -180,14 +179,13 @@ Definition eval_clstep_fulfil_def:
     | (SOME l, SOME v) =>
         (let
            (* The pre-view *)
-           v_pre = MAXL [ v_addr
-                          ; v_data
-                          ; s.bst_v_wNew
-                          ; s.bst_v_CAP
-                          ; ifView rel (MAX s.bst_v_rOld s.bst_v_wOld)
-                          ; ifView (xcl /\ acq /\ rel) s.bst_v_Rel
-                          ; ifView xcl (get_xclb_view s.bst_xclb)
-                        ];
+           v_pre = MAXL [v_addr;
+                         v_data;
+                         s.bst_v_wNew;
+                         s.bst_v_CAP;
+                         ifView rel (MAX s.bst_v_rOld s.bst_v_wOld);
+                         ifView (xcl /\ acq /\ rel) s.bst_v_Rel;
+                         ifView xcl (get_xclb_view s.bst_xclb)];
 
            (* The message to fulfil. *)
            msg = <| loc := l; val := v; cid := cid |>;
@@ -201,13 +199,13 @@ Definition eval_clstep_fulfil_def:
          in
            MAP_PARTIAL (\v_post. (* v_post = t *)
                           (* Updates the environ and viewenv if we have a store conditional *)
-                          case (fulfil_update_env p s xcl, fulfil_update_viewenv p s xcl v_post) of
+                          case (fulfil_update_env p s, fulfil_update_viewenv p s v_post) of
                           | (SOME new_env, SOME new_viewenv) => 
                               SOME ([v_post],
                                     s with <| bst_viewenv := new_viewenv;
                                               bst_environ := new_env;
                                               bst_prom   updated_by (FILTER (\t'. t' <> v_post));
-                                              bst_coh    updated_by (l =+ MAX (s.bst_coh l) v_post);
+                                              bst_coh    updated_by (l =+ v_post);
                                               bst_v_wOld updated_by MAX v_post;
                                               bst_v_CAP  updated_by MAX v_addr;
                                               bst_v_Rel  updated_by (MAX $ ifView (rel /\ acq) v_post);
@@ -232,8 +230,8 @@ End
  *   If xcl = T, then execute an xcl failure, a store-conditional that failed.
  *   Otherwise does nothing.
  *)
-Definition eval_clstep_xclfail_def:
-  (eval_clstep_xclfail p cid s T =
+Definition eval_clstep_store_xclfail_def:
+  (eval_clstep_store_xclfail p cid s T =
    case (xclfail_update_env p s, xclfail_update_viewenv p s) of
    | (SOME new_env, SOME new_viewenv) =>
        [([]: num list,
@@ -243,7 +241,7 @@ Definition eval_clstep_xclfail_def:
                    bst_pc updated_by (bir_pc_next o bir_pc_next o bir_pc_next) |>)]
    | _ => [])
   /\
-  eval_clstep_xclfail p cid s F = []
+  eval_clstep_store_xclfail p cid s F = []
 End
 
 (****************************************
@@ -253,14 +251,17 @@ End
  *   Implements our AMO fulfil rule.
  *   Basically a xcl read and fulfil without failure and xcl_bank.
  *)
-Definition eval_clstep_amofulfil_def:
-  eval_clstep_amofulfil cid s M var a_e v_e acq rel =
+Definition eval_clstep_amo_fulfil_def:
+  eval_clstep_amo_fulfil cid s M var a_e v_e acq rel =
   case bir_eval_exp_view a_e s.bst_environ s.bst_viewenv of
   | (NONE, v_addr) => []
   | (SOME l, v_addr) =>
       let
         (* Out read pre-view. *)
-        v_rPre = MAXL [v_addr; s.bst_v_rNew; ifView (acq /\ rel) s.bst_v_Rel; ifView (acq /\ rel) (MAX s.bst_v_rOld s.bst_v_wOld)];
+        v_rPre = MAXL [v_addr;
+                       s.bst_v_rNew;
+                       ifView (acq /\ rel) s.bst_v_Rel;
+                       ifView (acq /\ rel) (MAX s.bst_v_rOld s.bst_v_wOld)];
         (* Readable writes # timestamps. *)
         msgs = mem_readable M l (MAX v_rPre (s.bst_coh l));
       in                                 
@@ -303,7 +304,7 @@ Definition eval_clstep_amofulfil_def:
                                                                                      fwdb_view := MAX v_addr v_data;
                                                                                      fwdb_xcl  := T |>);
                                                       bst_prom   updated_by (FILTER (\t'. t' <> v_wPost));
-                                                      bst_coh    updated_by (l =+ MAX (s.bst_coh l) v_wPost);
+                                                      bst_coh    updated_by (l =+ v_wPost);
                                                       bst_v_Rel  updated_by (MAX (ifView (acq /\ rel) v_wPost));
                                                       bst_v_rOld updated_by (MAX v_rPost);
                                                       bst_v_rNew updated_by (MAX (ifView acq (if rel then v_wPost else v_rPost)));
@@ -343,13 +344,12 @@ End
 Definition eval_clstep_branch_def:
   eval_clstep_branch p s cond_e lbl1 lbl2 =
   let
-    stmt = BStmtE (BStmt_CJmp cond_e lbl1 lbl2);
     (sv, v_addr) = bir_eval_exp_view cond_e s.bst_environ s.bst_viewenv
   in
     case sv of
     | NONE => []
     | SOME v =>
-        let (oo,s2) = bir_exec_stmt p stmt s
+        let s2 = bir_exec_stmt_cjmp p cond_e lbl1 lbl2 s
         in [([]: num list,
              s2 with <| bst_v_CAP := MAX s.bst_v_CAP v_addr |>)]
 End
@@ -361,8 +361,8 @@ End
  *   Implements execution of an expression, the register rule.
  *   Mainly updates the register view.
  *)
-Definition eval_clstep_exp_def:
-  eval_clstep_exp s var ex =
+Definition eval_clstep_assign_def:
+  eval_clstep_assign s var ex =
   case bir_eval_exp_view ex s.bst_environ s.bst_viewenv
   of (SOME val, v_val) =>
        (case env_update_cast64 (bir_var_name var) val (bir_var_type var) (s.bst_environ) of
@@ -383,8 +383,9 @@ End
  *)
 Definition eval_clstep_bir_step_def:
   eval_clstep_bir_step p s stm =
-  let (oo,s') = bir_exec_stmt p stm s
-  in [([]: num list, s')]
+  case bmc_exec_general_stmt p stm s of
+       | SOME (oo, s') => [([]: num list, s')]
+       | NONE => []
 End
 
 (****************************************
@@ -396,27 +397,29 @@ End
  *)
 Definition eval_clstep_def:
   eval_clstep cid p s M =
-  case bir_get_stmt p s.bst_pc of
-  | BirStmt_Read var a_e cast_opt xcl acq rel =>
-      eval_clstep_read s M var a_e xcl acq rel
-  | BirStmt_Write a_e v_e xcl acq rel =>
-      eval_clstep_fulfil p cid s M a_e v_e xcl acq rel ++
-      eval_clstep_xclfail p cid s xcl
-  | BirStmt_Amo var a_e v_e acq rel =>
-      eval_clstep_amofulfil cid s M var a_e v_e acq rel
-  | BirStmt_Expr var e =>
-      eval_clstep_exp s var e
-  | BirStmt_Fence K1 K2 =>
+  if s.bst_status = BST_Running then
+  (case bir_get_current_statement p s.bst_pc of
+  | SOME (BStmtB (BMCStmt_Load var a_e cast_opt xcl acq rel)) =>
+      eval_clstep_load s M var a_e xcl acq rel
+  | SOME (BStmtB (BMCStmt_Store var_succ a_e v_e xcl acq rel)) =>
+      eval_clstep_store_fulfil p cid s M a_e v_e xcl acq rel ++
+      eval_clstep_store_xclfail p cid s xcl
+  | SOME (BStmtB (BMCStmt_Amo var a_e v_e acq rel)) =>
+      eval_clstep_amo_fulfil cid s M var a_e v_e acq rel
+  | SOME (BStmtB (BMCStmt_Assign var e)) =>
+      eval_clstep_assign s var e
+  | SOME (BStmtB (BMCStmt_Fence K1 K2)) =>
       eval_clstep_fence s K1 K2
-  | BirStmt_Branch cond_e lbl1 lbl2 =>
+  | SOME (BStmtE (BStmt_CJmp cond_e lbl1 lbl2)) =>
       eval_clstep_branch p s cond_e lbl1 lbl2
-  | BirStmt_Generic stm =>
+  | SOME stm =>
       eval_clstep_bir_step p s stm
-  | BirStmt_None => []
+  | NONE => [])
+  else []
 End
 
-Definition eval_cstep_seq_write_def:
-  eval_cstep_seq_write p cid s M a_e v_e xcl acq rel =
+Definition eval_cstep_seq_store_def:
+  eval_cstep_seq_store p cid s M a_e v_e xcl acq rel =
   let
     (val_opt, v_data) = bir_eval_exp_view v_e s.bst_environ s.bst_viewenv;
     (loc_opt, v_addr) = bir_eval_exp_view a_e s.bst_environ s.bst_viewenv;
@@ -424,18 +427,18 @@ Definition eval_cstep_seq_write_def:
     case (val_opt, loc_opt) of
     | (SOME v, SOME l) =>
         (let
-           msg = <| val := v; loc := l; cid := cid |>;
+           msg = <|val := v; loc := l; cid := cid|>;
            M' = SNOC msg M;
            t = LENGTH M';
            s' = s with <| bst_prom updated_by (SNOC t) |>;
          in
-           MAP (\ (l, s''). (s'', [msg])) (FILTER (\ (l,s''). l = [t]) (eval_clstep_fulfil p cid s' M' a_e v_e xcl acq rel))
+           MAP (\ (l, s''). (s'', [msg])) (FILTER (\ (l,s''). l = [t]) (eval_clstep_storefulfil p cid s' M' a_e v_e xcl acq rel))
         )
     | _ => []
 End
 
-Definition eval_cstep_seq_amowrite_def:
-  eval_cstep_seq_amowrite cid s M var a_e v_e acq rel =
+Definition eval_cstep_seq_amo_def:
+  eval_cstep_seq_amo cid s M var a_e v_e acq rel =
   case bir_eval_exp_view a_e s.bst_environ s.bst_viewenv of
   | (NONE, v_addr) => []
   | (SOME l, v_addr) =>
@@ -469,25 +472,27 @@ End
 
 Definition eval_cstep_seq_def:
   eval_cstep_seq cid p s M =
-  case bir_get_stmt p s.bst_pc of
-  | BirStmt_Read var a_e cast_opt xcl acq rel =>
-      MAP (\ (l,s'). (s', [])) (eval_clstep_read s M var a_e xcl acq rel)
-  | BirStmt_Write a_e v_e xcl acq rel =>
-      eval_cstep_seq_write p cid s M a_e v_e xcl acq rel ++
-      MAP (\ (l,s'). (s', [])) (eval_clstep_fulfil p cid s M a_e v_e xcl acq rel) ++
-      MAP (\ (l,s'). (s', [])) (eval_clstep_xclfail p cid s xcl)
-  | BirStmt_Amo var a_e v_e acq rel =>
-      eval_cstep_seq_amowrite cid s M var a_e v_e acq rel ++
-      MAP (\ (l,s'). (s', [])) (eval_clstep_amofulfil cid s M var a_e v_e acq rel)
-  | BirStmt_Expr var e =>
+  if s.bst_status = BST_Running then
+  (case bir_get_current_statement p s.bst_pc of
+  | SOME (BStmtB (BMCStmt_Load var a_e cast_opt xcl acq rel)) =>
+      MAP (\ (l,s'). (s', [])) (eval_clstep_load s M var a_e xcl acq rel)
+  | SOME (BStmtB (BMCStmt_Store var_succ a_e v_e xcl acq rel)) =>
+      eval_cstep_seq_store p cid s M a_e v_e xcl acq rel ++
+      MAP (\ (l,s'). (s', [])) (eval_clstep_store_fulfil p cid s M a_e v_e xcl acq rel) ++
+      MAP (\ (l,s'). (s', [])) (eval_clstep_store_xclfail p cid s xcl)
+  | SOME (BStmtB (BMCStmt_Amo var a_e v_e acq rel)) =>
+      eval_cstep_seq_amo cid s M var a_e v_e acq rel ++
+      MAP (\ (l,s'). (s', [])) (eval_clstep_amo_fulfil cid s M var a_e v_e acq rel)
+  | SOME (BStmtB (BMCStmt_Assign var e)) =>
       MAP (\ (l,s'). (s', [])) (eval_clstep_exp s var e)
-  | BirStmt_Fence K1 K2 =>
+  | SOME (BStmtB (BMCStmt_Fence K1 K2)) =>
       MAP (\ (l,s'). (s', [])) (eval_clstep_fence s K1 K2)
-  | BirStmt_Branch cond_e lbl1 lbl2 =>
+  | SOME (BStmtE (BStmt_CJmp cond_e lbl1 lbl2)) =>
       MAP (\ (l,s'). (s', [])) (eval_clstep_branch p s cond_e lbl1 lbl2)
-  | BirStmt_Generic stm =>
+  | SOME stm =>
       MAP (\ (l,s'). (s', [])) (eval_clstep_bir_step p s stm)
-  | BirStmt_None => []
+  | NONE => [])
+  else []
 End
 
 Definition eval_is_certified_def:
@@ -519,460 +524,6 @@ Definition eval_promstep_def:
          (eval_findprom f cid p s M)
 End
 
-(*
-(************************************************************
- * OPTIMIZED EXECUTABLE SEMANTICS 
- ************************************************************)
-
-(* This datatype has extra information for the promising execution *)
-val _ = Datatype‘
-         exec_core_t = ExecCore num (string bir_program_t) bir_state_t bool
-        ’;
-
-(* This datatype has extra information for the promising execution *)
-val _ = Datatype‘
-         exec_mem_msg_t = <| loc:bir_val_t ; val:bir_val_t ; cid:num ; succ:bool ; n:num |>
-        ’;
-
-val emem_default_def = Define‘
-  emem_default l = <| loc := l ; val := BVal_Imm (Imm64 0w) ; succ := T ; n := 0 |>
-’;
-
-val emem_get_def = Define‘
-  (emem_get M l 0 = SOME $ emem_default l)
-  /\
-  (emem_get M l (SUC t) = oEL t M)
-’;
-
-val emem_read_def = Define‘
-  emem_read M l t = OPTION_BIND (emem_get M l t) (λm. SOME m.val)
-’;
-
-val emem_filter_def = Define‘
-  emem_filter P M = FILTER P (ZIP(M,[1..LENGTH M]))
-’;
-
-val emem_every_def = Define‘
-  emem_every P M = EVERY P (ZIP(M,[1..LENGTH M]))
-’;
-
-val emem_readable_def = Define‘
-  emem_readable M l v_max =
-  FILTER (λ(m,t). emem_every (λ(m',t'). m'.succ /\ t < t' /\ t' <= v_max ==> m'.loc <> l) M)
-         ((emem_default l,0)::emem_filter (λ(m,t). m.loc = l /\ m.succ) M)
-’;
-
-val emem_atomic_def = Define‘
-  emem_atomic M l cid t_r t_w =
-  case emem_get M l t_r of
-  | SOME msg =>
-      msg.succ ==>
-      emem_every (λ(m,t'). t_r < t' /\ t' < t_w /\ m.loc = l /\ m.succ ==> m.cid = cid) M
-  | NONE => T
-’;
-
-val emem_to_mem_def = Define ‘
-  emem_to_mem [] = ([]: mem_msg_t list)
-  /\
-  (emem_to_mem (m::ms) =
-  if m.succ
-  then ((<| loc := m.loc; val := m.val; cid := m.cid |>)::emem_to_mem ms)
-  else emem_to_mem ms)
-’;
-
-val eval_clstep_readO1_def = Define‘
-  eval_clstep_readO1 s M var a_e xcl acq rel =
-  case bir_eval_exp_view a_e s.bst_environ s.bst_viewenv of
-  | (SOME l, v_addr) =>
-      let
-        v_pre = MAXL [ v_addr;
-                       s.bst_v_rNew;
-                       ifView (acq /\ rel) s.bst_v_Rel;
-                       ifView (acq /\ rel) (MAX s.bst_v_rOld s.bst_v_wOld)];
-        msgs  = emem_readable M l (MAX v_pre (s.bst_coh l)) 
-      in
-        MAP_PARTIAL (λ(msg,t).
-                          let
-                            v_post = MAX v_pre (mem_read_view (s.bst_fwdb(l)) t)
-                          in
-                            (case env_update_cast64 (bir_var_name var) msg.val (bir_var_type var) (s.bst_environ) of
-                             | SOME new_env =>
-                                 SOME (s with <| bst_environ := new_env;
-                                            bst_viewenv updated_by (λenv. FUPDATE env (var, v_post));
-                                            bst_coh     updated_by (l =+ MAX (s.bst_coh l) v_post);
-                                            bst_v_rOld  updated_by (MAX v_post);
-                                            bst_v_rNew  updated_by (MAX $ ifView acq v_post);
-                                            bst_v_wNew  updated_by (MAX $ ifView acq v_post);
-                                            bst_v_Rel   updated_by (MAX $ ifView (rel /\ acq) v_post);
-                                            bst_v_CAP   updated_by (MAX v_addr);
-                                            bst_pc      updated_by if xcl
-                                                                   then (bir_pc_next o bir_pc_next)
-                                                                   else bir_pc_next;
-                                            bst_xclb    := if xcl
-                                                           then SOME <| xclb_time := t; xclb_view := v_post |>
-                                                           else s.bst_xclb |>)
-                             | NONE => NONE)) msgs
-        | _ => []
-’;
-
-(* Optimized fulfil *)
-val eval_clstep_fulfilO1_def = Define‘
-  eval_clstep_fulfilO1 p cid s M a_e v_e xcl acq rel =
-  let
-    (val_opt, v_data) = bir_eval_exp_view v_e s.bst_environ s.bst_viewenv;
-    (loc_opt, v_addr) = bir_eval_exp_view a_e s.bst_environ s.bst_viewenv;
-  in
-    case (val_opt, loc_opt) of
-    | (SOME v, SOME l) =>
-        (let
-           msg = <| val := v; loc := l; cid := cid; n := SUC s.bst_counter |>;
-           v_pre = MAXL [ v_addr ; v_data ; s.bst_v_wNew ; s.bst_v_CAP;
-                          ifView rel (MAX s.bst_v_rOld s.bst_v_wOld);
-                          ifView (xcl /\ acq /\ rel) s.bst_v_Rel;
-                          ifView xcl (get_xclb_view s.bst_xclb)];
-           (* Candidate t's *)
-           ts = FILTER (\t. (emem_get M l t = SOME msg) /\
-                            (MAX v_pre (s.bst_coh l) < t) /\
-                            (xcl ==> (IS_SOME s.bst_xclb) /\
-                                     emem_atomic M l cid (THE s.bst_xclb).xclb_time t))
-                       s.bst_prom
-         in
-           MAP_PARTIAL (λv_post.
-                          case (fulfil_update_env p s xcl, fulfil_update_viewenv p s xcl v_post) of
-                          | (SOME new_env, SOME new_viewenv) => 
-                              SOME (s with <| bst_viewenv := new_viewenv;
-                                              bst_environ := new_env;
-                                              bst_prom   updated_by (FILTER (\t'. t' <> v_post));
-                                              bst_coh    updated_by (l =+ MAX (s.bst_coh l) v_post);
-                                              bst_v_wOld updated_by MAX v_post;
-                                              bst_v_CAP  updated_by MAX v_addr;
-                                              bst_v_Rel  updated_by MAX (ifView (rel /\ acq) v_post);
-                                              bst_v_rNew updated_by MAX (ifView (rel /\ acq /\ xcl) v_post);
-                                              bst_v_wNew updated_by MAX (ifView (rel /\ acq /\ xcl) v_post);
-                                              bst_fwdb   updated_by (l =+ <| fwdb_time := v_post;
-                                                                             fwdb_view := MAX v_addr v_data;
-                                                                             fwdb_xcl := xcl |>);
-                                              bst_pc     updated_by if xcl
-                                                                    then (bir_pc_next o bir_pc_next o bir_pc_next)
-                                                                    else bir_pc_next;
-                                              bst_counter updated_by SUC;
-                                              bst_xclb := if xcl then NONE else s.bst_xclb |>)
-                          | _ => NONE
-                       ) ts
-        )
-    | _ => []
-’;
-
-(* Optimized xclfail *)
-val eval_clstep_xclfailO1_def = Define‘
-  (eval_clstep_xclfailO1 p cid s M a_e v_e T =
-   case (xclfail_update_env p s, xclfail_update_viewenv p s) of
-   | (SOME new_env, SOME new_viewenv) =>
-       [s with <| bst_viewenv := new_viewenv;
-                  bst_environ := new_env;
-                  bst_xclb    := NONE;
-                  bst_counter updated_by SUC;
-                  bst_pc      updated_by (bir_pc_next o bir_pc_next o bir_pc_next) |>]
-   | _ => [])
-  /\
-  eval_clstep_xclfailO1 p cid s M a_e v_e F = []
-’;
-
-val eval_clstep_amofulfilO1_def = Define‘
-  eval_clstep_amofulfilO1 cid s M var a_e v_e acq rel =
-  case bir_eval_exp_view a_e s.bst_environ s.bst_viewenv of
-  | (NONE, v_addr) => []
-  | (SOME l, v_addr) =>
-      let
-        v_rPre = MAXL [v_addr; s.bst_v_rNew; ifView (acq /\ rel) s.bst_v_Rel; ifView (acq /\ rel) (MAX s.bst_v_rOld s.bst_v_wOld)];
-        msgs = emem_readable M l (MAX v_rPre (s.bst_coh l));
-      in                                 
-        LIST_BIND msgs
-                  (\ (msg,t_r).
-                     let
-                       v_rPost = MAX v_rPre (mem_read_view (s.bst_fwdb l) t_r);
-                       new_viewenv = FUPDATE s.bst_viewenv (var, v_rPost);
-                     in
-                       (case env_update_cast64 (bir_var_name var) msg.val (bir_var_type var) (s.bst_environ) of
-                        | NONE => []
-                        | SOME new_environ =>
-                            (case bir_eval_exp_view v_e new_environ new_viewenv of
-                             | (NONE, v_data) => []
-                             | (SOME v, v_data) =>
-                                 let
-                                   v_wPre = MAXL [v_addr; v_data; s.bst_v_CAP; v_rPost; s.bst_v_wNew;
-                                                  ifView rel (MAX s.bst_v_rOld s.bst_v_wOld);
-                                                  ifView (acq /\ rel) s.bst_v_Rel];
-                                   msg = <| loc := l; val := v; cid := cid ; succ := T; n := SUC s.bst_counter |>;
-                                   t_ws = FILTER (\t_w.
-                                                    (emem_get M l t_w = SOME msg) /\
-                                                    (MAX v_wPre (s.bst_coh l) < t_w) /\
-                                                    (emem_every (\ (msg,t'). msg.succ /\ t_r < t' /\ t' < t_w ==> msg.loc <> l) M))
-                                                 s.bst_prom;
-                                 in LIST_BIND t_ws (\v_wPost.
-                                                      [ s with <| bst_viewenv := new_viewenv;
-                                                                  bst_environ := new_environ;
-                                                                  bst_fwdb   updated_by (l =+ <| fwdb_time := v_wPost;
-                                                                                                 fwdb_view := MAX v_addr v_data;
-                                                                                                 fwdb_xcl  := T |>);
-                                                                  bst_prom   updated_by (FILTER (\t'. t' <> v_wPost));
-                                                                  bst_coh    updated_by (l =+ MAX (s.bst_coh l) v_wPost);
-                                                                  bst_v_Rel  updated_by (MAX (ifView (acq /\ rel) v_wPost));
-                                                                  bst_v_rOld updated_by (MAX v_rPost);
-                                                                  bst_v_rNew updated_by (MAX (ifView acq (if rel then v_wPost else v_rPost)));
-                                                                  bst_v_wNew updated_by (MAX (ifView acq (if rel then v_wPost else v_rPost)));
-                                                                  bst_v_CAP  updated_by (MAX v_addr);
-                                                                  bst_v_wOld updated_by (MAX v_wPost);
-                                                                  bst_pc     updated_by bir_pc_next o bir_pc_next;
-                                                               |> ])
-                            )
-                       )
-                  )
-’;
-
-(* Optimized clstep *)
-val eval_clstepO1_def = Define‘
-  eval_clstepO1 p cid s M =
-    case bir_get_stmt p s.bst_pc of
-    | BirStmt_Read var a_e cast_opt xcl acq rel =>
-        eval_clstep_readO1 s M var a_e xcl acq rel
-    | BirStmt_Write a_e v_e xcl acq rel =>
-        eval_clstep_fulfilO1 p cid s M a_e v_e xcl acq rel ++
-        eval_clstep_xclfailO1 p cid s M a_e v_e xcl
-    | BirStmt_Amo var a_e v_e acq rel =>
-        eval_clstep_amofulfilO1 cid s M var a_e v_e acq rel
-    | BirStmt_Expr var e =>
-        eval_clstep_exp s var e
-    | BirStmt_Fence K1 K2 =>
-        eval_clstep_fence s K1 K2
-    | BirStmt_Branch cond_e lbl1 lbl2 =>
-        eval_clstep_branch p s cond_e lbl1 lbl2
-    | BirStmt_Generic stm =>
-        eval_clstep_bir_step p s stm
-    | BirStmt_None => []
-’;
-
-(* Optimized clsteps *)
-val eval_clstepsO1_def = Define‘
-  (
-  eval_clstepsO1 0 cid p s M =
-  case s.bst_status of
-  | BST_Running => [s]
-  | BST_Halted _ => [s]
-  | BST_JumpOutside _ => [s]
-  | _ => []
-  ) /\ (
-  eval_clstepsO1 (SUC f) cid p s M = 
-  case s.bst_status of
-  | BST_Running => LIST_BIND (eval_clstepO1 p cid s M)
-                             (\s'. eval_clstepsO1 f cid p s' M)
-  | BST_Halted _ => [s]
-  | BST_JumpOutside _ => [s]
-  | _ => []
-  )
-’;
-
-val eval_clsteps_coreO1_def = Define‘
-  eval_clsteps_coreO1 fuel (Core cid prog st) M =
-    MAP (\st'. Core cid prog st') (eval_clstepsO1 fuel cid prog st M)
-’;
-
-val eval_certifyO1_def = Define‘
-  (
-  eval_certifyO1 prog cid st M 0 =
-  NULL st.bst_prom
-  ) /\ (
-  eval_certifyO1 prog cid st M (SUC f) =
-  (NULL st.bst_prom \/
-   EXISTS (λst'. eval_certifyO1 prog cid st' M f) (eval_clstepO1 prog cid st M))
-  )
-’;
-
-val eval_certify_coreO1_def = Define‘
-  eval_certify_coreO1 M f (Core cid prog st) =
-  eval_certifyO1 prog cid st M f
-’;
-
-(**** Promising mode execution, optimized ****)
-
-val has_write = Define‘
-  has_write M cid n = EXISTS (\m. m.cid = cid /\ m.n = n) M
-’;
-
-(* Find promise write step (promise-step + fulfil) *)
-val eval_fpstep_writeO1_def = Define‘
-  eval_fpstep_writeO1 p cid s M a_e v_e xcl acq rel =
-  if ~has_write M cid (SUC s.bst_counter) then
-  let
-    (val_opt, v_data) = bir_eval_exp_view v_e s.bst_environ s.bst_viewenv;
-    (loc_opt, v_addr) = bir_eval_exp_view a_e s.bst_environ s.bst_viewenv;
-  in
-    case (val_opt, loc_opt) of
-    | (SOME v, SOME l) =>
-        (let
-           msg = <| val := v; loc := l; cid := cid; succ := T; n := SUC s.bst_counter |>;
-           M' = SNOC msg M;
-           s' = s with <| bst_prom updated_by (CONS (LENGTH M')) |>;
-           v_prom = MAXL [ v_addr; v_data; s.bst_v_wNew; s.bst_v_CAP
-                         ; if rel then (MAX s.bst_v_rOld s.bst_v_wOld) else 0
-                         ; if (xcl /\ acq /\ rel) then s.bst_v_Rel else 0
-                         ; if xcl then get_xclb_view s.bst_xclb else 0
-                         ; s.bst_coh l
-                         ];
-         in
-           MAP (\s''. (SOME (msg, v_prom), s''))
-               (eval_clstep_fulfilO1 p cid s' M' a_e v_e xcl acq rel)
-        )
-    | _ => []
-  else []
-’;
-
-val eval_fpstep_amowriteO1_def = Define‘
-  eval_fpstep_amowriteO1 cid s M var a_e v_e acq rel =
-  if ~has_write M cid (SUC s.bst_counter) then
-    case bir_eval_exp_view a_e s.bst_environ s.bst_viewenv of
-    | (NONE, v_addr) => []
-    | (SOME l, v_addr) =>
-        let
-          v_rPre = MAXL [v_addr; s.bst_v_rNew; ifView (acq /\ rel) s.bst_v_Rel];
-          msgs = emem_readable M l (MAX v_rPre (s.bst_coh l));
-        in                                 
-          LIST_BIND msgs
-                    (\ (msg,t_r).
-                       let
-                         v_rPost = MAX v_rPre (mem_read_view (s.bst_fwdb l) t_r);
-                         new_viewenv = FUPDATE s.bst_viewenv (var, v_rPost);
-                       in
-                         case env_update_cast64 (bir_var_name var) msg.val (bir_var_type var) (s.bst_environ) of
-                         | NONE => []
-                         | SOME new_environ =>
-                             (case bir_eval_exp_view v_e new_environ new_viewenv of
-                              | (NONE, v_data) => []
-                              | (SOME v, v_data) =>
-                                  let
-                                    msg = <| loc := l; val := v; cid := cid ; succ := T ; n := (SUC s.bst_counter) |>;
-                                    M' = SNOC msg M;
-                                    s' = s with <| bst_prom updated_by (CONS (LENGTH M')) |>;
-                                    v_post = MAXL [v_addr; v_data; s.bst_v_CAP; v_rPost; s.bst_v_wNew;
-                                                   ifView rel (MAX s.bst_v_rOld s.bst_v_wOld);
-                                                   ifView (acq /\ rel) s.bst_v_Rel;
-                                                   s.bst_coh l
-                                                  ];
-                                  in
-                                    map (\s''. (SOME (msg, v_post), s''))
-                                        (eval_clstep_amofulfilO1 cid s' M' var a_e v_e acq rel)
-                             )
-                    )
-  else []
-’;
-
-(* Find promise step *)
-val eval_fpstepO1_def = Define‘
-  eval_fpstepO1 p cid s M =
-    case bir_get_stmt p s.bst_pc of
-    | BirStmt_Read var a_e cast_opt xcl acq rel =>
-        MAP (\s. (NONE,s)) (eval_clstep_readO1 s M var a_e xcl acq rel)
-    | BirStmt_Write a_e v_e xcl acq rel =>
-        (MAP (\s. (NONE,s)) (eval_clstep_fulfilO1 p cid s M a_e v_e xcl acq rel)) ++
-        (MAP (\s. (NONE,s)) (eval_clstep_xclfailO1 p cid s M a_e v_e xcl)) ++
-        (eval_fpstep_writeO1 p cid s M a_e v_e xcl acq rel)
-    | BirStmt_Amo var a_e v_e acq rel =>
-        (MAP (\s. (NONE,s)) (eval_clstep_amofulfilO1 cid s M var a_e v_e acq rel)) ++
-        (eval_fpstep_amowriteO1 cid s M var a_e v_e acq rel)
-    | BirStmt_Expr var e =>
-        MAP (\s. (NONE,s)) (eval_clstep_exp s var e)
-    | BirStmt_Fence K1 K2 =>
-        MAP (\s. (NONE,s)) (eval_clstep_fence s K1 K2)
-    | BirStmt_Branch cond_e lbl1 lbl2 =>
-        MAP (\s. (NONE,s)) (eval_clstep_branch p s cond_e lbl1 lbl2)
-    | BirStmt_Generic stm =>
-        MAP (\s. (NONE,s)) (eval_clstep_bir_step p s stm)
-    | BirStmt_None => []
-’;
-
-(* Find promise steps *)
-val eval_fpstepsO1_def = Define‘
-  (
-  eval_fpstepsO1 0 (t:num) prog cid st M prom =
-  if NULL st.bst_prom then prom else []
-  ) /\ (
-  eval_fpstepsO1 (SUC fuel) t prog cid st M prom = 
-  case st.bst_status of
-  | BST_Running =>
-      LIST_BIND (eval_fpstepO1 prog cid st M)
-                (λ(msg_opt,st').
-                   case msg_opt of
-                   | SOME (msg, v_prom) =>
-                       let
-                         prom' = if v_prom < t then (msg::prom) else prom;
-                         M' = SNOC msg M
-                       in eval_fpstepsO1 fuel t prog cid st' M' prom'
-                   | NONE => eval_fpstepsO1 fuel t prog cid st' M prom)
-  | BST_Halted _ =>
-      if NULL st.bst_prom then prom else []
-  | BST_JumpOutside _ =>
-      if NULL st.bst_prom then prom else []
-  | _ => []
-  )
-’;
-
-(* Find promise steps on a core *)
-val eval_fpsteps_coreO1_def = Define‘
-  eval_fpsteps_coreO1 fuel (Core cid prog st) M =
-    eval_fpstepsO1 fuel (SUC (LENGTH M)) prog cid st M []
-’;
-
-(* Find all next promises-steps *)
-val eval_find_promisesO1_def = Define‘
-  eval_find_promisesO1 fuel (cores, M) =
-  LIST_BIND cores (λcore. eval_fpsteps_coreO1 fuel core M)
-’;
-
-val eval_make_promise_auxO1_def = Define‘
-  eval_make_promise_auxO1 msg t (Core cid prog st) =
-  if msg.cid = cid
-  then (Core cid prog (st with <| bst_prom updated_by (CONS t) |>))
-  else (Core cid prog st) 
-’;
-
-val eval_make_promiseO1_def = Define‘
-  eval_make_promiseO1 (cores,M) msg =
-  let M' = SNOC msg M;
-      t = LENGTH M';
-      cores' = MAP (eval_make_promise_auxO1 msg t) cores
-    in (cores', M')
-’;
-
-
-(* Promise-mode step *)
-val eval_pmstepO1_def = Define‘
-  eval_pmstepO1 fuel (cores, M) =
-  let promises = nub $ eval_find_promisesO1 fuel (cores, M);
-  in MAP (eval_make_promiseO1 (cores,M)) promises
-’;
-
-val eval_pmstepsO1_def = Define‘
-  eval_pmstepsO1 fuel 0 cM = [cM]
-  /\
-  eval_pmstepsO1 fuel (SUC pfuel) cM =
-  let cMs = eval_pmstepO1 fuel cM in
-  if NULL cMs
-  then [cM]
-  else LIST_BIND cMs (eval_pmstepsO1 fuel pfuel)
-’;
-
-val eval_finished_def = Define‘
-  eval_finished s =
-  case s.bst_status of
-  | BST_Halted v => NULL s.bst_prom
-  | BST_JumpOutside l => NULL s.bst_prom
-  | _ => F
-’;
-
-val eval_finished_core_def = Define‘
-  eval_finished_core (Core cid prog s) = eval_finished s
-’;
-*)
 
 (****************************************
  * THEOREM: EL_SNOC2
@@ -1259,15 +810,14 @@ Proof
   ]
 QED
 
-
 Theorem MEM_readable_thm:
   ∀m_t M v_max l.
   MEM m_t (mem_readable M l v_max)
   = (mem_get M l (SND m_t) = SOME (FST m_t) ∧
-     ∀t'. (SND m_t) < t' ∧ t' ≤ v_max ⇒ ~mem_is_loc M t' l)
+     ∀t'. latest_t l M (SND m_t) v_max)
 Proof
   tmCases_on “m_t” ["m t"] >>
-  fs [] >>
+  fs [latest_t_def] >>
   rpt gen_tac >>
   eq_tac >|
   [
@@ -1324,20 +874,22 @@ QED
  * Soundness proof of executable core-local step
  ************************************************************)
 
-Theorem eval_clstep_read_soundness:
+Theorem eval_clstep_load_soundness:
   ∀p cid M s s' var e acq rel xcl cast l.
-  MEM (l, s') (eval_clstep_read s M var e acq rel xcl) ==>
-  bir_get_stmt p s.bst_pc = BirStmt_Read var e cast acq rel xcl ==>
+  s.bst_status = BST_Running ∧
+  MEM (l, s') (eval_clstep_load s M var e acq rel xcl) ==>
+  bir_get_current_statement p s.bst_pc = SOME (BStmtB (BMCStmt_Load var e cast acq rel xcl)) ==>
   clstep p cid s M l s'
 Proof
   rpt strip_tac >>
-  fs [eval_clstep_read_def, bir_eval_exp_view_def] >>
+  fs [eval_clstep_load_def, bir_eval_exp_view_def] >>
   Cases_on ‘bir_eval_exp e s.bst_environ’ >- (fs [CaseEq"option"]) >>
   fs [CaseEq"option"] >>
   fs [MEM_MAP_PARTIAL, MEM_MAP] >>
   rename1 ‘MEM msg_t (mem_readable M loc _)’ >> tmCases_on “msg_t” ["msg t"] >>
   fs [MEM_readable_thm] >>
   fs [clstep_cases, bir_state_t_component_equality, bir_eval_exp_view_def] >>
+  DISJ1_TAC >>
   imp_res_tac mem_get_mem_read >>
   Q.EXISTS_TAC ‘msg.val’ >> Q.EXISTS_TAC ‘t’ >>
   fs [MAXL_def, ifView_def, combinTheory.UPDATE_def] >>
@@ -1345,51 +897,54 @@ Proof
   (rfs [] >> METIS_TAC [MAX_COMM, MAX_ASSOC])
 QED                                   
 
-Theorem eval_clstep_fulfil_soundness:
-  ∀p s s' a_e v_e xcl acq rel cid M l.
-  bir_get_stmt p s.bst_pc = BirStmt_Write a_e v_e xcl acq rel ==>
-  MEM (l, s') (eval_clstep_fulfil p cid s M a_e v_e xcl acq rel) ==>
+Theorem eval_clstep_store_fulfil_soundness:
+  ∀p s s' var_succ a_e v_e xcl acq rel cid M l.
+  s.bst_status = BST_Running ∧
+  bir_get_current_statement p s.bst_pc = SOME (BStmtB (BMCStmt_Store var_succ a_e v_e xcl acq rel)) ∧
+  MEM (l, s') (eval_clstep_store_fulfil p cid s M a_e v_e xcl acq rel) ⇒
   clstep p cid s M l s'
 Proof
   rpt strip_tac >>
-  fs [eval_clstep_fulfil_def, bir_eval_exp_view_def] >>
+  fs [eval_clstep_store_fulfil_def, bir_eval_exp_view_def] >>
   tmCases_on “bir_eval_exp a_e s.bst_environ” ["", "loc"] >> fs[] >>
   tmCases_on “bir_eval_exp v_e s.bst_environ” ["", "val"] >> fs[] >>
   fs [MEM_MAP_PARTIAL, MEM_MAP, MEM_FILTER] >>
-  tmCases_on “fulfil_update_env p s xcl” ["", "new_env"] >> fs [] >>
-  tmCases_on “fulfil_update_viewenv p s xcl v_post” ["", "new_viewenv"] >> fs [] >>
+  tmCases_on “fulfil_update_env p s” ["", "new_env"] >> fs [] >>
+  tmCases_on “fulfil_update_viewenv p s v_post” ["", "new_viewenv"] >> fs [] >>
   fs [clstep_cases, bir_eval_exp_view_def, bir_state_t_component_equality, combinTheory.UPDATE_def,
       mem_atomic_correctness, MAXL_def, ifView_def, IS_SOME_EQ_NOT_NONE] >>
   Cases_on ‘xcl’ >> Cases_on ‘acq’ >> Cases_on ‘rel’ >> fs [] >> METIS_TAC [MAX_COMM]
 QED
 
-Theorem eval_clstep_xclfail_soundness:
-  ∀p s s' a_e v_e xcl acq rel cid M l.
-  bir_get_stmt p s.bst_pc = BirStmt_Write a_e v_e xcl acq rel ==>
-  MEM (l, s') (eval_clstep_xclfail p cid s xcl) ==>
+Theorem eval_clstep_store_xclfail_soundness:
+  ∀p s s' var_succ a_e v_e xcl acq rel cid M l.
+  s.bst_status = BST_Running ∧
+  bir_get_current_statement p s.bst_pc = SOME (BStmtB (BMCStmt_Store var_succ a_e v_e xcl acq rel)) ∧
+  MEM (l, s') (eval_clstep_store_xclfail p cid s xcl) ⇒
   clstep p cid s M l s'
 Proof
   rpt strip_tac >>
   Cases_on ‘xcl’ >|
   [
-    fs [eval_clstep_xclfail_def, clstep_cases] >>
+    fs [eval_clstep_store_xclfail_def, clstep_cases] >>
     Cases_on ‘xclfail_update_env p s’ >- (fs []) >>
     Cases_on ‘xclfail_update_viewenv p s’ >- (fs []) >>
     rpt strip_tac >>
     fs [bir_state_t_component_equality]
     ,
-    fs [eval_clstep_xclfail_def]
+    fs [eval_clstep_store_xclfail_def]
   ]
 QED
 
-Theorem eval_clstep_amofulfil_soundness:
+Theorem eval_clstep_amo_fulfil_soundness:
   ∀p s var a_e v_e acq rel s' cid M l.
-  MEM (l, s') (eval_clstep_amofulfil cid s M var a_e v_e acq rel) ==>
-  bir_get_stmt p s.bst_pc = BirStmt_Amo var a_e v_e acq rel ==>
+  s.bst_status = BST_Running ∧
+  MEM (l, s') (eval_clstep_amo_fulfil cid s M var a_e v_e acq rel) ∧
+  bir_get_current_statement p s.bst_pc = SOME (BStmtB (BMCStmt_Amo var a_e v_e acq rel)) ⇒
   clstep p cid s M l s'
 Proof
   rpt strip_tac >>
-  fs [eval_clstep_amofulfil_def, bir_eval_exp_view_def] >>
+  fs [eval_clstep_amo_fulfil_def, bir_eval_exp_view_def] >>
   tmCases_on “bir_eval_exp a_e s.bst_environ” ["", "loc"] >> fs [] >>
   fs [LIST_BIND_def, MEM_FLAT] >>
   rename1 ‘MEM (l, s') state_list’ >>
@@ -1408,21 +963,23 @@ Proof
   Cases_on ‘acq’ >> Cases_on ‘rel’ >> fs []
 QED
 
-Theorem eval_clstep_expr_soundness:
+Theorem eval_clstep_assign_soundness:
   ∀p cid M s s' var e l.
-  MEM (l, s') (eval_clstep_exp s var e) ==>
-  bir_get_stmt p s.bst_pc = BirStmt_Expr var e ==>
+  s.bst_status = BST_Running ∧
+  MEM (l, s') (eval_clstep_assign s var e) ∧
+  bir_get_current_statement p s.bst_pc = SOME (BStmtB (BMCStmt_Assign var e)) ==>
   clstep p cid s M l s'
 Proof
   rpt strip_tac >>
-  fs [clstep_cases, eval_clstep_exp_def] >>
-  rpt (FULL_CASE_TAC >> fs [bir_get_stmt_expr])
+  fs [clstep_cases, eval_clstep_assign_def] >>
+  rpt (FULL_CASE_TAC >> fs [])
 QED                                              
 
 Theorem eval_clstep_fence_soundness:
   ∀p cid M s s' K1 K2 l.
-  bir_get_stmt p s.bst_pc = BirStmt_Fence K1 K2 ==>
-  MEM (l, s') (eval_clstep_fence s K1 K2) ==>
+  s.bst_status = BST_Running ∧
+  bir_get_current_statement p s.bst_pc = SOME (BStmtB (BMCStmt_Fence K1 K2)) ∧
+  MEM (l, s') (eval_clstep_fence s K1 K2) ⇒
   clstep p cid s M l s'
 Proof
   rpt strip_tac >>
@@ -1433,29 +990,30 @@ QED
 
 Theorem eval_clstep_branch_soundness:
   ∀p cid M s s' cond_e lbl1 lbl2 l.
-  bir_get_stmt p s.bst_pc = BirStmt_Branch cond_e lbl1 lbl2 ==>
-  MEM (l,s') (eval_clstep_branch p s cond_e lbl1 lbl2) ==>
+  s.bst_status = BST_Running ∧
+  bir_get_current_statement p s.bst_pc = SOME (BStmtE (BStmt_CJmp cond_e lbl1 lbl2)) ∧
+  MEM (l,s') (eval_clstep_branch p s cond_e lbl1 lbl2) ⇒
   clstep p cid s M l s'
 Proof
   rpt strip_tac >>
   fs [clstep_cases, eval_clstep_branch_def, bir_state_t_component_equality] >>
-  Cases_on ‘bir_exec_stmt p (BStmtE (BStmt_CJmp cond_e lbl1 lbl2)) s’ >>
   Cases_on ‘bir_eval_exp_view cond_e s.bst_environ s.bst_viewenv’ >>
   fs [] >>
-  FULL_CASE_TAC >>
-  (fs [])
+  FULL_CASE_TAC >> (fs [])
 QED
+
 
 Theorem eval_clstep_generic_soundness:
   ∀p cid M s s' stmt l.
-  bir_get_stmt p s.bst_pc = BirStmt_Generic stmt ==>
+  s.bst_status = BST_Running ∧
+  bir_get_current_statement p s.bst_pc = SOME stmt ==>
   MEM (l,s') (eval_clstep_bir_step p s stmt) ==>
   clstep p cid s M l s'
 Proof
   rpt strip_tac >>
   fs [clstep_cases, eval_clstep_bir_step_def, bir_state_t_component_equality] >>
-  Cases_on ‘bir_exec_stmt p stmt s’ >>
-  fs []
+  fs [bmc_exec_general_stmt_def] >>
+  rpt (FULL_CASE_TAC >> fs[])
 QED
 
 Theorem eval_clstep_soundness:
@@ -1465,21 +1023,39 @@ Theorem eval_clstep_soundness:
 Proof
   rpt strip_tac
   >> fs [eval_clstep_def]
-  >> Cases_on ‘bir_get_stmt p s.bst_pc’
+  >> Cases_on ‘s.bst_status = BST_Running’
   >| [
-    fs [eval_clstep_read_soundness]
-    ,
-    fs [eval_clstep_fulfil_soundness, eval_clstep_xclfail_soundness]
-    ,
-    fs [eval_clstep_amofulfil_soundness]
-    ,
-    fs [eval_clstep_expr_soundness]
-    ,
-    fs [eval_clstep_fence_soundness]
-    ,
-    fs [eval_clstep_branch_soundness]
-    ,
-    fs [eval_clstep_generic_soundness]
+    Cases_on ‘bir_get_current_statement p s.bst_pc’ >> fs[] >>
+    FULL_CASE_TAC
+    >| [ (* BStmtB *)
+      fs [] >>
+      FULL_CASE_TAC >|
+      [ (* load *)
+        fs [eval_clstep_load_soundness]
+        , (* store *)
+        fs [eval_clstep_store_fulfil_soundness, eval_clstep_store_xclfail_soundness]
+        , (* amo *)
+        fs [eval_clstep_amo_fulfil_soundness]
+        , (* assign *)
+        fs [eval_clstep_assign_soundness]
+        , (* fence *)
+        fs [eval_clstep_fence_soundness]
+        , (* assert *)
+        fs [eval_clstep_generic_soundness]
+        , (* assume *)
+        fs [eval_clstep_generic_soundness]
+      ]
+      , (* BStmtE *)
+      fs [] >>
+      FULL_CASE_TAC >|
+      [ (* jmp *)
+        fs [eval_clstep_generic_soundness]
+        , (* cjmp *)
+        fs [eval_clstep_branch_soundness]
+        , (* halt *)
+        fs [eval_clstep_generic_soundness]
+      ]
+    ]
     ,
     fs []
   ]
@@ -2140,5 +1716,460 @@ val _ = Hol_reln `
   (!l. mem_get M l i = mem_get M' l j)
   ==> sim cid i j (s,M) (s',M'))
 `;
+
+(*
+(************************************************************
+ * OPTIMIZED EXECUTABLE SEMANTICS 
+ ************************************************************)
+
+(* This datatype has extra information for the promising execution *)
+val _ = Datatype‘
+         exec_core_t = ExecCore num (string bir_program_t) bir_state_t bool
+        ’;
+
+(* This datatype has extra information for the promising execution *)
+val _ = Datatype‘
+         exec_mem_msg_t = <| loc:bir_val_t ; val:bir_val_t ; cid:num ; succ:bool ; n:num |>
+        ’;
+
+val emem_default_def = Define‘
+  emem_default l = <| loc := l ; val := BVal_Imm (Imm64 0w) ; succ := T ; n := 0 |>
+’;
+
+val emem_get_def = Define‘
+  (emem_get M l 0 = SOME $ emem_default l)
+  /\
+  (emem_get M l (SUC t) = oEL t M)
+’;
+
+val emem_read_def = Define‘
+  emem_read M l t = OPTION_BIND (emem_get M l t) (λm. SOME m.val)
+’;
+
+val emem_filter_def = Define‘
+  emem_filter P M = FILTER P (ZIP(M,[1..LENGTH M]))
+’;
+
+val emem_every_def = Define‘
+  emem_every P M = EVERY P (ZIP(M,[1..LENGTH M]))
+’;
+
+val emem_readable_def = Define‘
+  emem_readable M l v_max =
+  FILTER (λ(m,t). emem_every (λ(m',t'). m'.succ /\ t < t' /\ t' <= v_max ==> m'.loc <> l) M)
+         ((emem_default l,0)::emem_filter (λ(m,t). m.loc = l /\ m.succ) M)
+’;
+
+val emem_atomic_def = Define‘
+  emem_atomic M l cid t_r t_w =
+  case emem_get M l t_r of
+  | SOME msg =>
+      msg.succ ==>
+      emem_every (λ(m,t'). t_r < t' /\ t' < t_w /\ m.loc = l /\ m.succ ==> m.cid = cid) M
+  | NONE => T
+’;
+
+val emem_to_mem_def = Define ‘
+  emem_to_mem [] = ([]: mem_msg_t list)
+  /\
+  (emem_to_mem (m::ms) =
+  if m.succ
+  then ((<| loc := m.loc; val := m.val; cid := m.cid |>)::emem_to_mem ms)
+  else emem_to_mem ms)
+’;
+
+val eval_clstep_readO1_def = Define‘
+  eval_clstep_readO1 s M var a_e xcl acq rel =
+  case bir_eval_exp_view a_e s.bst_environ s.bst_viewenv of
+  | (SOME l, v_addr) =>
+      let
+        v_pre = MAXL [ v_addr;
+                       s.bst_v_rNew;
+                       ifView (acq /\ rel) s.bst_v_Rel;
+                       ifView (acq /\ rel) (MAX s.bst_v_rOld s.bst_v_wOld)];
+        msgs  = emem_readable M l (MAX v_pre (s.bst_coh l)) 
+      in
+        MAP_PARTIAL (λ(msg,t).
+                          let
+                            v_post = MAX v_pre (mem_read_view (s.bst_fwdb(l)) t)
+                          in
+                            (case env_update_cast64 (bir_var_name var) msg.val (bir_var_type var) (s.bst_environ) of
+                             | SOME new_env =>
+                                 SOME (s with <| bst_environ := new_env;
+                                            bst_viewenv updated_by (λenv. FUPDATE env (var, v_post));
+                                            bst_coh     updated_by (l =+ MAX (s.bst_coh l) v_post);
+                                            bst_v_rOld  updated_by (MAX v_post);
+                                            bst_v_rNew  updated_by (MAX $ ifView acq v_post);
+                                            bst_v_wNew  updated_by (MAX $ ifView acq v_post);
+                                            bst_v_Rel   updated_by (MAX $ ifView (rel /\ acq) v_post);
+                                            bst_v_CAP   updated_by (MAX v_addr);
+                                            bst_pc      updated_by if xcl
+                                                                   then (bir_pc_next o bir_pc_next)
+                                                                   else bir_pc_next;
+                                            bst_xclb    := if xcl
+                                                           then SOME <| xclb_time := t; xclb_view := v_post |>
+                                                           else s.bst_xclb |>)
+                             | NONE => NONE)) msgs
+        | _ => []
+’;
+
+(* Optimized fulfil *)
+val eval_clstep_fulfilO1_def = Define‘
+  eval_clstep_fulfilO1 p cid s M a_e v_e xcl acq rel =
+  let
+    (val_opt, v_data) = bir_eval_exp_view v_e s.bst_environ s.bst_viewenv;
+    (loc_opt, v_addr) = bir_eval_exp_view a_e s.bst_environ s.bst_viewenv;
+  in
+    case (val_opt, loc_opt) of
+    | (SOME v, SOME l) =>
+        (let
+           msg = <| val := v; loc := l; cid := cid; n := SUC s.bst_counter |>;
+           v_pre = MAXL [ v_addr ; v_data ; s.bst_v_wNew ; s.bst_v_CAP;
+                          ifView rel (MAX s.bst_v_rOld s.bst_v_wOld);
+                          ifView (xcl /\ acq /\ rel) s.bst_v_Rel;
+                          ifView xcl (get_xclb_view s.bst_xclb)];
+           (* Candidate t's *)
+           ts = FILTER (\t. (emem_get M l t = SOME msg) /\
+                            (MAX v_pre (s.bst_coh l) < t) /\
+                            (xcl ==> (IS_SOME s.bst_xclb) /\
+                                     emem_atomic M l cid (THE s.bst_xclb).xclb_time t))
+                       s.bst_prom
+         in
+           MAP_PARTIAL (λv_post.
+                          case (fulfil_update_env p s xcl, fulfil_update_viewenv p s xcl v_post) of
+                          | (SOME new_env, SOME new_viewenv) => 
+                              SOME (s with <| bst_viewenv := new_viewenv;
+                                              bst_environ := new_env;
+                                              bst_prom   updated_by (FILTER (\t'. t' <> v_post));
+                                              bst_coh    updated_by (l =+ MAX (s.bst_coh l) v_post);
+                                              bst_v_wOld updated_by MAX v_post;
+                                              bst_v_CAP  updated_by MAX v_addr;
+                                              bst_v_Rel  updated_by MAX (ifView (rel /\ acq) v_post);
+                                              bst_v_rNew updated_by MAX (ifView (rel /\ acq /\ xcl) v_post);
+                                              bst_v_wNew updated_by MAX (ifView (rel /\ acq /\ xcl) v_post);
+                                              bst_fwdb   updated_by (l =+ <| fwdb_time := v_post;
+                                                                             fwdb_view := MAX v_addr v_data;
+                                                                             fwdb_xcl := xcl |>);
+                                              bst_pc     updated_by if xcl
+                                                                    then (bir_pc_next o bir_pc_next o bir_pc_next)
+                                                                    else bir_pc_next;
+                                              bst_counter updated_by SUC;
+                                              bst_xclb := if xcl then NONE else s.bst_xclb |>)
+                          | _ => NONE
+                       ) ts
+        )
+    | _ => []
+’;
+
+(* Optimized xclfail *)
+val eval_clstep_xclfailO1_def = Define‘
+  (eval_clstep_xclfailO1 p cid s M a_e v_e T =
+   case (xclfail_update_env p s, xclfail_update_viewenv p s) of
+   | (SOME new_env, SOME new_viewenv) =>
+       [s with <| bst_viewenv := new_viewenv;
+                  bst_environ := new_env;
+                  bst_xclb    := NONE;
+                  bst_counter updated_by SUC;
+                  bst_pc      updated_by (bir_pc_next o bir_pc_next o bir_pc_next) |>]
+   | _ => [])
+  /\
+  eval_clstep_xclfailO1 p cid s M a_e v_e F = []
+’;
+
+val eval_clstep_amofulfilO1_def = Define‘
+  eval_clstep_amofulfilO1 cid s M var a_e v_e acq rel =
+  case bir_eval_exp_view a_e s.bst_environ s.bst_viewenv of
+  | (NONE, v_addr) => []
+  | (SOME l, v_addr) =>
+      let
+        v_rPre = MAXL [v_addr; s.bst_v_rNew; ifView (acq /\ rel) s.bst_v_Rel; ifView (acq /\ rel) (MAX s.bst_v_rOld s.bst_v_wOld)];
+        msgs = emem_readable M l (MAX v_rPre (s.bst_coh l));
+      in                                 
+        LIST_BIND msgs
+                  (\ (msg,t_r).
+                     let
+                       v_rPost = MAX v_rPre (mem_read_view (s.bst_fwdb l) t_r);
+                       new_viewenv = FUPDATE s.bst_viewenv (var, v_rPost);
+                     in
+                       (case env_update_cast64 (bir_var_name var) msg.val (bir_var_type var) (s.bst_environ) of
+                        | NONE => []
+                        | SOME new_environ =>
+                            (case bir_eval_exp_view v_e new_environ new_viewenv of
+                             | (NONE, v_data) => []
+                             | (SOME v, v_data) =>
+                                 let
+                                   v_wPre = MAXL [v_addr; v_data; s.bst_v_CAP; v_rPost; s.bst_v_wNew;
+                                                  ifView rel (MAX s.bst_v_rOld s.bst_v_wOld);
+                                                  ifView (acq /\ rel) s.bst_v_Rel];
+                                   msg = <| loc := l; val := v; cid := cid ; succ := T; n := SUC s.bst_counter |>;
+                                   t_ws = FILTER (\t_w.
+                                                    (emem_get M l t_w = SOME msg) /\
+                                                    (MAX v_wPre (s.bst_coh l) < t_w) /\
+                                                    (emem_every (\ (msg,t'). msg.succ /\ t_r < t' /\ t' < t_w ==> msg.loc <> l) M))
+                                                 s.bst_prom;
+                                 in LIST_BIND t_ws (\v_wPost.
+                                                      [ s with <| bst_viewenv := new_viewenv;
+                                                                  bst_environ := new_environ;
+                                                                  bst_fwdb   updated_by (l =+ <| fwdb_time := v_wPost;
+                                                                                                 fwdb_view := MAX v_addr v_data;
+                                                                                                 fwdb_xcl  := T |>);
+                                                                  bst_prom   updated_by (FILTER (\t'. t' <> v_wPost));
+                                                                  bst_coh    updated_by (l =+ MAX (s.bst_coh l) v_wPost);
+                                                                  bst_v_Rel  updated_by (MAX (ifView (acq /\ rel) v_wPost));
+                                                                  bst_v_rOld updated_by (MAX v_rPost);
+                                                                  bst_v_rNew updated_by (MAX (ifView acq (if rel then v_wPost else v_rPost)));
+                                                                  bst_v_wNew updated_by (MAX (ifView acq (if rel then v_wPost else v_rPost)));
+                                                                  bst_v_CAP  updated_by (MAX v_addr);
+                                                                  bst_v_wOld updated_by (MAX v_wPost);
+                                                                  bst_pc     updated_by bir_pc_next o bir_pc_next;
+                                                               |> ])
+                            )
+                       )
+                  )
+’;
+
+(* Optimized clstep *)
+val eval_clstepO1_def = Define‘
+  eval_clstepO1 p cid s M =
+    case bir_get_stmt p s.bst_pc of
+    | BirStmt_Read var a_e cast_opt xcl acq rel =>
+        eval_clstep_readO1 s M var a_e xcl acq rel
+    | BirStmt_Write a_e v_e xcl acq rel =>
+        eval_clstep_fulfilO1 p cid s M a_e v_e xcl acq rel ++
+        eval_clstep_xclfailO1 p cid s M a_e v_e xcl
+    | BirStmt_Amo var a_e v_e acq rel =>
+        eval_clstep_amofulfilO1 cid s M var a_e v_e acq rel
+    | BirStmt_Expr var e =>
+        eval_clstep_exp s var e
+    | BirStmt_Fence K1 K2 =>
+        eval_clstep_fence s K1 K2
+    | BirStmt_Branch cond_e lbl1 lbl2 =>
+        eval_clstep_branch p s cond_e lbl1 lbl2
+    | BirStmt_Generic stm =>
+        eval_clstep_bir_step p s stm
+    | BirStmt_None => []
+’;
+
+(* Optimized clsteps *)
+val eval_clstepsO1_def = Define‘
+  (
+  eval_clstepsO1 0 cid p s M =
+  case s.bst_status of
+  | BST_Running => [s]
+  | BST_Halted _ => [s]
+  | BST_JumpOutside _ => [s]
+  | _ => []
+  ) /\ (
+  eval_clstepsO1 (SUC f) cid p s M = 
+  case s.bst_status of
+  | BST_Running => LIST_BIND (eval_clstepO1 p cid s M)
+                             (\s'. eval_clstepsO1 f cid p s' M)
+  | BST_Halted _ => [s]
+  | BST_JumpOutside _ => [s]
+  | _ => []
+  )
+’;
+
+val eval_clsteps_coreO1_def = Define‘
+  eval_clsteps_coreO1 fuel (Core cid prog st) M =
+    MAP (\st'. Core cid prog st') (eval_clstepsO1 fuel cid prog st M)
+’;
+
+val eval_certifyO1_def = Define‘
+  (
+  eval_certifyO1 prog cid st M 0 =
+  NULL st.bst_prom
+  ) /\ (
+  eval_certifyO1 prog cid st M (SUC f) =
+  (NULL st.bst_prom \/
+   EXISTS (λst'. eval_certifyO1 prog cid st' M f) (eval_clstepO1 prog cid st M))
+  )
+’;
+
+val eval_certify_coreO1_def = Define‘
+  eval_certify_coreO1 M f (Core cid prog st) =
+  eval_certifyO1 prog cid st M f
+’;
+
+(**** Promising mode execution, optimized ****)
+
+val has_write = Define‘
+  has_write M cid n = EXISTS (\m. m.cid = cid /\ m.n = n) M
+’;
+
+(* Find promise write step (promise-step + fulfil) *)
+val eval_fpstep_writeO1_def = Define‘
+  eval_fpstep_writeO1 p cid s M a_e v_e xcl acq rel =
+  if ~has_write M cid (SUC s.bst_counter) then
+  let
+    (val_opt, v_data) = bir_eval_exp_view v_e s.bst_environ s.bst_viewenv;
+    (loc_opt, v_addr) = bir_eval_exp_view a_e s.bst_environ s.bst_viewenv;
+  in
+    case (val_opt, loc_opt) of
+    | (SOME v, SOME l) =>
+        (let
+           msg = <| val := v; loc := l; cid := cid; succ := T; n := SUC s.bst_counter |>;
+           M' = SNOC msg M;
+           s' = s with <| bst_prom updated_by (CONS (LENGTH M')) |>;
+           v_prom = MAXL [ v_addr; v_data; s.bst_v_wNew; s.bst_v_CAP
+                         ; if rel then (MAX s.bst_v_rOld s.bst_v_wOld) else 0
+                         ; if (xcl /\ acq /\ rel) then s.bst_v_Rel else 0
+                         ; if xcl then get_xclb_view s.bst_xclb else 0
+                         ; s.bst_coh l
+                         ];
+         in
+           MAP (\s''. (SOME (msg, v_prom), s''))
+               (eval_clstep_fulfilO1 p cid s' M' a_e v_e xcl acq rel)
+        )
+    | _ => []
+  else []
+’;
+
+val eval_fpstep_amowriteO1_def = Define‘
+  eval_fpstep_amowriteO1 cid s M var a_e v_e acq rel =
+  if ~has_write M cid (SUC s.bst_counter) then
+    case bir_eval_exp_view a_e s.bst_environ s.bst_viewenv of
+    | (NONE, v_addr) => []
+    | (SOME l, v_addr) =>
+        let
+          v_rPre = MAXL [v_addr; s.bst_v_rNew; ifView (acq /\ rel) s.bst_v_Rel];
+          msgs = emem_readable M l (MAX v_rPre (s.bst_coh l));
+        in                                 
+          LIST_BIND msgs
+                    (\ (msg,t_r).
+                       let
+                         v_rPost = MAX v_rPre (mem_read_view (s.bst_fwdb l) t_r);
+                         new_viewenv = FUPDATE s.bst_viewenv (var, v_rPost);
+                       in
+                         case env_update_cast64 (bir_var_name var) msg.val (bir_var_type var) (s.bst_environ) of
+                         | NONE => []
+                         | SOME new_environ =>
+                             (case bir_eval_exp_view v_e new_environ new_viewenv of
+                              | (NONE, v_data) => []
+                              | (SOME v, v_data) =>
+                                  let
+                                    msg = <| loc := l; val := v; cid := cid ; succ := T ; n := (SUC s.bst_counter) |>;
+                                    M' = SNOC msg M;
+                                    s' = s with <| bst_prom updated_by (CONS (LENGTH M')) |>;
+                                    v_post = MAXL [v_addr; v_data; s.bst_v_CAP; v_rPost; s.bst_v_wNew;
+                                                   ifView rel (MAX s.bst_v_rOld s.bst_v_wOld);
+                                                   ifView (acq /\ rel) s.bst_v_Rel;
+                                                   s.bst_coh l
+                                                  ];
+                                  in
+                                    map (\s''. (SOME (msg, v_post), s''))
+                                        (eval_clstep_amofulfilO1 cid s' M' var a_e v_e acq rel)
+                             )
+                    )
+  else []
+’;
+
+(* Find promise step *)
+val eval_fpstepO1_def = Define‘
+  eval_fpstepO1 p cid s M =
+    case bir_get_stmt p s.bst_pc of
+    | BirStmt_Read var a_e cast_opt xcl acq rel =>
+        MAP (\s. (NONE,s)) (eval_clstep_readO1 s M var a_e xcl acq rel)
+    | BirStmt_Write a_e v_e xcl acq rel =>
+        (MAP (\s. (NONE,s)) (eval_clstep_fulfilO1 p cid s M a_e v_e xcl acq rel)) ++
+        (MAP (\s. (NONE,s)) (eval_clstep_xclfailO1 p cid s M a_e v_e xcl)) ++
+        (eval_fpstep_writeO1 p cid s M a_e v_e xcl acq rel)
+    | BirStmt_Amo var a_e v_e acq rel =>
+        (MAP (\s. (NONE,s)) (eval_clstep_amofulfilO1 cid s M var a_e v_e acq rel)) ++
+        (eval_fpstep_amowriteO1 cid s M var a_e v_e acq rel)
+    | BirStmt_Expr var e =>
+        MAP (\s. (NONE,s)) (eval_clstep_exp s var e)
+    | BirStmt_Fence K1 K2 =>
+        MAP (\s. (NONE,s)) (eval_clstep_fence s K1 K2)
+    | BirStmt_Branch cond_e lbl1 lbl2 =>
+        MAP (\s. (NONE,s)) (eval_clstep_branch p s cond_e lbl1 lbl2)
+    | BirStmt_Generic stm =>
+        MAP (\s. (NONE,s)) (eval_clstep_bir_step p s stm)
+    | BirStmt_None => []
+’;
+
+(* Find promise steps *)
+val eval_fpstepsO1_def = Define‘
+  (
+  eval_fpstepsO1 0 (t:num) prog cid st M prom =
+  if NULL st.bst_prom then prom else []
+  ) /\ (
+  eval_fpstepsO1 (SUC fuel) t prog cid st M prom = 
+  case st.bst_status of
+  | BST_Running =>
+      LIST_BIND (eval_fpstepO1 prog cid st M)
+                (λ(msg_opt,st').
+                   case msg_opt of
+                   | SOME (msg, v_prom) =>
+                       let
+                         prom' = if v_prom < t then (msg::prom) else prom;
+                         M' = SNOC msg M
+                       in eval_fpstepsO1 fuel t prog cid st' M' prom'
+                   | NONE => eval_fpstepsO1 fuel t prog cid st' M prom)
+  | BST_Halted _ =>
+      if NULL st.bst_prom then prom else []
+  | BST_JumpOutside _ =>
+      if NULL st.bst_prom then prom else []
+  | _ => []
+  )
+’;
+
+(* Find promise steps on a core *)
+val eval_fpsteps_coreO1_def = Define‘
+  eval_fpsteps_coreO1 fuel (Core cid prog st) M =
+    eval_fpstepsO1 fuel (SUC (LENGTH M)) prog cid st M []
+’;
+
+(* Find all next promises-steps *)
+val eval_find_promisesO1_def = Define‘
+  eval_find_promisesO1 fuel (cores, M) =
+  LIST_BIND cores (λcore. eval_fpsteps_coreO1 fuel core M)
+’;
+
+val eval_make_promise_auxO1_def = Define‘
+  eval_make_promise_auxO1 msg t (Core cid prog st) =
+  if msg.cid = cid
+  then (Core cid prog (st with <| bst_prom updated_by (CONS t) |>))
+  else (Core cid prog st) 
+’;
+
+val eval_make_promiseO1_def = Define‘
+  eval_make_promiseO1 (cores,M) msg =
+  let M' = SNOC msg M;
+      t = LENGTH M';
+      cores' = MAP (eval_make_promise_auxO1 msg t) cores
+    in (cores', M')
+’;
+
+
+(* Promise-mode step *)
+val eval_pmstepO1_def = Define‘
+  eval_pmstepO1 fuel (cores, M) =
+  let promises = nub $ eval_find_promisesO1 fuel (cores, M);
+  in MAP (eval_make_promiseO1 (cores,M)) promises
+’;
+
+val eval_pmstepsO1_def = Define‘
+  eval_pmstepsO1 fuel 0 cM = [cM]
+  /\
+  eval_pmstepsO1 fuel (SUC pfuel) cM =
+  let cMs = eval_pmstepO1 fuel cM in
+  if NULL cMs
+  then [cM]
+  else LIST_BIND cMs (eval_pmstepsO1 fuel pfuel)
+’;
+
+val eval_finished_def = Define‘
+  eval_finished s =
+  case s.bst_status of
+  | BST_Halted v => NULL s.bst_prom
+  | BST_JumpOutside l => NULL s.bst_prom
+  | _ => F
+’;
+
+val eval_finished_core_def = Define‘
+  eval_finished_core (Core cid prog s) = eval_finished s
+’;
+*)
 
 val _ = export_theory();
